<?xml version="1.0"?>
<rdf:RDF xmlns="http://www.semanticweb.org/ipro#"
     xml:base="http://www.semanticweb.org/ipro"
     xmlns:dc="http://purl.org/dc/elements/1.1/"
     xmlns:owl="http://www.w3.org/2002/07/owl#"
     xmlns:rdf="http://www.w3.org/1999/02/22-rdf-syntax-ns#"
     xmlns:xml="http://www.w3.org/XML/1998/namespace"
     xmlns:xsd="http://www.w3.org/2001/XMLSchema#"
     xmlns:foaf="http://xmlns.com/foaf/0.1/"
     xmlns:rdfs="http://www.w3.org/2000/01/rdf-schema#"
     xmlns:time="http://www.w3.org/2006/time#"
     xmlns:vann="http://purl.org/vocab/vann/"
     xmlns:cpannotationschema="http://www.ontologydesignpatterns.org/schemas/cpannotationschema.owl#">
    <owl:Ontology rdf:about="http://ipro-semantic.com">
        <owl:imports rdf:resource="http://www.ontologydesignpatterns.org/cp/owl/list.owl"/>
        <dc:creator rdf:datatype="http://www.w3.org/2001/XMLSchema#string">Davide Zago</dc:creator>
        <dc:date rdf:datatype="http://www.w3.org/2001/XMLSchema#integer">2022</dc:date>
        <dc:description xml:lang="en">IPRO (Italian Progressive Rock Ontology) is a semantic resource that represents the genre of Progressive Rock in Italy from 1966 to 1976. Although it&apos;s not an exhaustive resource, in contains various information about bands, albums, tracks, musicians, instruments and genres.</dc:description>
        <dc:title rdf:datatype="http://www.w3.org/2001/XMLSchema#string">IPRO</dc:title>
        <vann:preferredNamespacePrefix>ipro</vann:preferredNamespacePrefix>
        <vann:preferredNamespaceUri>http://ipro-semantic.com</vann:preferredNamespaceUri>
        <rdfs:label xml:lang="en">Italian Progressive Rock Ontology</rdfs:label>
    </owl:Ontology>
    


    <!-- 
    ///////////////////////////////////////////////////////////////////////////////////////
    //
    // Annotation properties
    //
    ///////////////////////////////////////////////////////////////////////////////////////
     -->

    


    <!-- http://purl.org/dc/elements/1.1/creator -->

    <owl:AnnotationProperty rdf:about="http://purl.org/dc/elements/1.1/creator"/>
    


    <!-- http://purl.org/dc/elements/1.1/date -->

    <owl:AnnotationProperty rdf:about="http://purl.org/dc/elements/1.1/date"/>
    


    <!-- http://purl.org/dc/elements/1.1/description -->

    <owl:AnnotationProperty rdf:about="http://purl.org/dc/elements/1.1/description"/>
    


    <!-- http://purl.org/dc/elements/1.1/title -->

    <owl:AnnotationProperty rdf:about="http://purl.org/dc/elements/1.1/title"/>
    


    <!-- http://purl.org/vocab/vann/preferredNamespacePrefix -->

    <owl:AnnotationProperty rdf:about="http://purl.org/vocab/vann/preferredNamespacePrefix"/>
    


    <!-- http://purl.org/vocab/vann/preferredNamespaceUri -->

    <owl:AnnotationProperty rdf:about="http://purl.org/vocab/vann/preferredNamespaceUri"/>
    


    <!-- 
    ///////////////////////////////////////////////////////////////////////////////////////
    //
    // Object Properties
    //
    ///////////////////////////////////////////////////////////////////////////////////////
     -->

    


    <!-- http://ipro-semantic.com#ofAlbum -->

    <owl:ObjectProperty rdf:about="http://ipro-semantic.com#ofAlbum">
        <rdfs:subPropertyOf rdf:resource="http://www.ontologydesignpatterns.org/cp/owl/bag.owl#itemContent"/>
        <rdf:type rdf:resource="http://www.w3.org/2002/07/owl#FunctionalProperty"/>
        <rdf:type rdf:resource="http://www.w3.org/2002/07/owl#InverseFunctionalProperty"/>
        <rdfs:domain rdf:resource="http://ipro-semantic.com#Release"/>
        <rdfs:range rdf:resource="http://ipro-semantic.com#Album"/>
        <rdfs:comment xml:lang="en">link from a release to the corresponding album</rdfs:comment>
        <rdfs:label xml:lang="en">of album</rdfs:label>
    </owl:ObjectProperty>
    


    <!-- http://www.w3.org/2006/time#hasDuration -->

    <owl:ObjectProperty rdf:about="http://www.w3.org/2006/time#hasDuration">
        <rdfs:range rdf:resource="http://www.w3.org/2006/time#DurationDescription"/>
    </owl:ObjectProperty>
    


    <!-- 
    ///////////////////////////////////////////////////////////////////////////////////////
    //
    // Data properties
    //
    ///////////////////////////////////////////////////////////////////////////////////////
     -->

    


    <!-- http://www.w3.org/2006/time#minutes -->

    <owl:DatatypeProperty rdf:about="http://www.w3.org/2006/time#minutes">
        <rdfs:domain rdf:resource="http://www.w3.org/2006/time#DurationDescription"/>
        <rdfs:range rdf:resource="http://www.w3.org/2001/XMLSchema#decimal"/>
    </owl:DatatypeProperty>
    


    <!-- http://www.w3.org/2006/time#seconds -->

    <owl:DatatypeProperty rdf:about="http://www.w3.org/2006/time#seconds">
        <rdfs:domain rdf:resource="http://www.w3.org/2006/time#DurationDescription"/>
        <rdfs:range rdf:resource="http://www.w3.org/2001/XMLSchema#decimal"/>
    </owl:DatatypeProperty>
    


    <!-- 
    ///////////////////////////////////////////////////////////////////////////////////////
    //
    // Classes
    //
    ///////////////////////////////////////////////////////////////////////////////////////
     -->

    


    <!-- http://ipro-semantic.com#Album -->

    <owl:Class rdf:about="http://ipro-semantic.com#Album">
        <rdfs:subClassOf rdf:resource="http://www.ontologydesignpatterns.org/cp/owl/list.owl#List"/>
        <rdfs:comment xml:lang="en">An album is a list of tracks composed by an artist or a band. An album typically contains 2 to 10-15 tracks. The typical total duration of an album is from 25 to 40 minutes, which has been limited to the writable surface of a vinyl record.</rdfs:comment>
        <rdfs:label xml:lang="en">Album</rdfs:label>
    </owl:Class>
    


    <!-- http://ipro-semantic.com#Band -->

    <owl:Class rdf:about="http://ipro-semantic.com#Band">
        <rdfs:comment xml:lang="en">Group of musicians who play music. A band is typically composed of 2 to 10 members. A band of more than 10 members is more frequently considered an orchestra, or a complex. The term band is often referred to popular music genres such as pop, rock, punk, metal, country and many more.</rdfs:comment>
        <rdfs:label xml:lang="en">Band</rdfs:label>
    </owl:Class>
    


    <!-- http://ipro-semantic.com#Bass -->

    <owl:Class rdf:about="http://ipro-semantic.com#Bass">
        <rdfs:subClassOf rdf:resource="http://ipro-semantic.com#StringsPlucked"/>
        <rdfs:comment xml:lang="en">A bass is a stringed musical instrument similar to a guitar but with lower notes. This category includes many variants of the bass.</rdfs:comment>
        <rdfs:label xml:lang="en">Bass</rdfs:label>
    </owl:Class>
    


    <!-- http://ipro-semantic.com#Bassist -->

    <owl:Class rdf:about="http://ipro-semantic.com#Bassist">
        <rdfs:subClassOf rdf:resource="http://ipro-semantic.com#Musician"/>
        <rdfs:comment xml:lang="en">Musician that plays the bass instrument.</rdfs:comment>
        <rdfs:label xml:lang="en">Bassist</rdfs:label>
    </owl:Class>
    


    <!-- http://ipro-semantic.com#BrassInstrument -->

    <owl:Class rdf:about="http://ipro-semantic.com#BrassInstrument">
        <rdfs:subClassOf rdf:resource="http://ipro-semantic.com#MusicalInstrument"/>
        <rdfs:comment xml:lang="en">A brass instrument is a musical instrument, typically a wind instrument, which is made out of brass.</rdfs:comment>
        <rdfs:label xml:lang="en">Brass instrument</rdfs:label>
    </owl:Class>
    


    <!-- http://ipro-semantic.com#Discography -->

    <owl:Class rdf:about="http://ipro-semantic.com#Discography">
        <rdfs:subClassOf rdf:resource="http://www.ontologydesignpatterns.org/cp/owl/list.owl#List"/>
        <rdfs:comment xml:lang="en">A discography is a list of releases published by an artist or a band. It is usually composed of studio albums, live albums and singles.</rdfs:comment>
        <rdfs:label xml:lang="en">Discography</rdfs:label>
    </owl:Class>
    


    <!-- http://ipro-semantic.com#Drummer -->

    <owl:Class rdf:about="http://ipro-semantic.com#Drummer">
        <rdfs:subClassOf rdf:resource="http://ipro-semantic.com#Musician"/>
        <rdfs:comment xml:lang="en">Musician that plays drums or percussion instruments</rdfs:comment>
        <rdfs:label xml:lang="en">Drummer</rdfs:label>
        <rdfs:label xml:lang="en">Percussionist</rdfs:label>
    </owl:Class>
    


    <!-- http://ipro-semantic.com#Drums -->

    <owl:Class rdf:about="http://ipro-semantic.com#Drums">
        <rdfs:subClassOf rdf:resource="http://ipro-semantic.com#PercussionInstrument"/>
        <rdfs:comment xml:lang="en">Drums (or drum kit) are one of the most common percussion instruments and it is a collection of different drums. The drum kit is very popular in genres such as rock, pop, punk, metal, and many more.</rdfs:comment>
        <rdfs:label xml:lang="en">Drums / drum kit</rdfs:label>
    </owl:Class>
    


    <!-- http://ipro-semantic.com#Effects -->

    <owl:Class rdf:about="http://ipro-semantic.com#Effects">
        <rdfs:subClassOf rdf:resource="http://ipro-semantic.com#MusicalInstrument"/>
        <rdfs:comment xml:lang="en">General effect used to play music</rdfs:comment>
        <rdfs:label xml:lang="en">Effects</rdfs:label>
    </owl:Class>
    


    <!-- http://ipro-semantic.com#Genre -->

    <owl:Class rdf:about="http://ipro-semantic.com#Genre">
        <rdfs:comment xml:lang="en">A genre is a term used to describe music with similarities, such as: similar or same instruments, similar rhythm, tempo, harmonies and melodies, and so on. A genre typically derive from one or more genres and it is strongly related to the place it originated from.</rdfs:comment>
        <rdfs:label xml:lang="en">Genre</rdfs:label>
    </owl:Class>
    


    <!-- http://ipro-semantic.com#Guitar -->

    <owl:Class rdf:about="http://ipro-semantic.com#Guitar">
        <rdfs:subClassOf rdf:resource="http://ipro-semantic.com#StringsPlucked"/>
        <rdfs:comment xml:lang="en">A guitar is a stringed musical instrument with many variants. It is typically played by plucking the strings</rdfs:comment>
        <rdfs:label xml:lang="en">Guitar</rdfs:label>
    </owl:Class>
    


    <!-- http://ipro-semantic.com#Guitarist -->

    <owl:Class rdf:about="http://ipro-semantic.com#Guitarist">
        <rdfs:subClassOf rdf:resource="http://ipro-semantic.com#Musician"/>
        <rdfs:comment xml:lang="en">Musician that plays the guitar.</rdfs:comment>
        <rdfs:label xml:lang="en">Guitarist</rdfs:label>
    </owl:Class>
    


    <!-- http://ipro-semantic.com#Keyboard -->

    <owl:Class rdf:about="http://ipro-semantic.com#Keyboard">
        <rdfs:subClassOf rdf:resource="http://ipro-semantic.com#MusicalInstrument"/>
        <rdfs:comment xml:lang="en">A keyboard is a musical instrument with keys. A keyboard player presses the keys to play  sound an music.</rdfs:comment>
        <rdfs:label xml:lang="en">Keyboard</rdfs:label>
    </owl:Class>
    


    <!-- http://ipro-semantic.com#Keyboardist -->

    <owl:Class rdf:about="http://ipro-semantic.com#Keyboardist">
        <rdfs:subClassOf rdf:resource="http://ipro-semantic.com#Musician"/>
        <rdfs:comment xml:lang="en">Musician that plays the keyboards.</rdfs:comment>
        <rdfs:label xml:lang="en">Keyboardist</rdfs:label>
    </owl:Class>
    


    <!-- http://ipro-semantic.com#MusicalInstrument -->

    <owl:Class rdf:about="http://ipro-semantic.com#MusicalInstrument">
        <rdfs:comment xml:lang="en">A musical instrument is an instrument used to play music</rdfs:comment>
        <rdfs:label xml:lang="en">Musical instrument</rdfs:label>
    </owl:Class>
    


    <!-- http://ipro-semantic.com#Musician -->

    <owl:Class rdf:about="http://ipro-semantic.com#Musician">
        <rdfs:comment xml:lang="en">A person who plays a musical instrument, especially as a profession, or is musically talented.</rdfs:comment>
        <rdfs:label xml:lang="en">Musician</rdfs:label>
    </owl:Class>
    


    <!-- http://ipro-semantic.com#Organ -->

    <owl:Class rdf:about="http://ipro-semantic.com#Organ">
        <rdfs:subClassOf rdf:resource="http://ipro-semantic.com#Keyboard"/>
        <rdfs:comment xml:lang="en">An organ is a keyboard with an unique sound. The main categories of organs are pipe organs and electric organs, which have very different sounds.</rdfs:comment>
        <rdfs:label xml:lang="en">Organ</rdfs:label>
    </owl:Class>
    


    <!-- http://ipro-semantic.com#Participation -->

    <owl:Class rdf:about="http://ipro-semantic.com#Participation">
        <rdfs:comment xml:lang="en">Participation of a musician to an album. The participation can be with a list of instruments or with roles in the production of the piece of music.</rdfs:comment>
        <rdfs:label xml:lang="en">Participation</rdfs:label>
    </owl:Class>
    


    <!-- http://ipro-semantic.com#PercussionInstrument -->

    <owl:Class rdf:about="http://ipro-semantic.com#PercussionInstrument">
        <rdfs:subClassOf rdf:resource="http://ipro-semantic.com#MusicalInstrument"/>
        <rdfs:comment xml:lang="en">A percussion instrument is a musical instrument which produces sound by being hit or struck.</rdfs:comment>
        <rdfs:label xml:lang="en">Percussion instrument</rdfs:label>
    </owl:Class>
    


    <!-- http://ipro-semantic.com#Percussions -->

    <owl:Class rdf:about="http://ipro-semantic.com#Percussions">
        <rdfs:subClassOf rdf:resource="http://ipro-semantic.com#PercussionInstrument"/>
        <rdfs:comment xml:lang="en">Percussions include a set of various percussion instruments that are not commonly identified as a drum kit.</rdfs:comment>
        <rdfs:label xml:lang="en">Percussions</rdfs:label>
    </owl:Class>
    


    <!-- http://ipro-semantic.com#Piano -->

    <owl:Class rdf:about="http://ipro-semantic.com#Piano">
        <rdfs:subClassOf rdf:resource="http://ipro-semantic.com#Keyboard"/>
        <rdfs:comment xml:lang="en">A piano is a keyboard where the key press triggers a hammer that strikes a string. Every key has one hammer. The piano is one of the most known musical instruments.</rdfs:comment>
        <rdfs:label xml:lang="en">Piano</rdfs:label>
    </owl:Class>
    


    <!-- http://ipro-semantic.com#ProductionRole -->

    <owl:Class rdf:about="http://ipro-semantic.com#ProductionRole">
        <rdfs:comment xml:lang="en">Generic role of a musician in a piece of music that is not strictly playing an instrument.</rdfs:comment>
        <rdfs:label xml:lang="en">Production role</rdfs:label>
    </owl:Class>
    


    <!-- http://ipro-semantic.com#Release -->

    <owl:Class rdf:about="http://ipro-semantic.com#Release">
        <rdfs:subClassOf rdf:resource="http://www.ontologydesignpatterns.org/cp/owl/list.owl#ListItem"/>
        <rdfs:comment xml:lang="en">A release is a publication of an album (or single) by a band. A release is part of a discography.</rdfs:comment>
        <rdfs:label xml:lang="en">Release</rdfs:label>
    </owl:Class>
    


    <!-- http://ipro-semantic.com#Singer -->

    <owl:Class rdf:about="http://ipro-semantic.com#Singer">
        <rdfs:subClassOf rdf:resource="http://ipro-semantic.com#Musician"/>
        <rdfs:comment xml:lang="en">Musician that sings / has vocal parts in a piece of music.</rdfs:comment>
        <rdfs:label xml:lang="en">Singer</rdfs:label>
    </owl:Class>
    


    <!-- http://ipro-semantic.com#Strings -->

    <owl:Class rdf:about="http://ipro-semantic.com#Strings">
        <rdfs:subClassOf rdf:resource="http://ipro-semantic.com#MusicalInstrument"/>
        <rdfs:comment xml:lang="en">Strings include a set of musical instruments with strings. A stringed instrument can be played by plucking or drawing the strings, which makes them vibrate and produce sound.</rdfs:comment>
        <rdfs:label xml:lang="en">Strings</rdfs:label>
    </owl:Class>
    


    <!-- http://ipro-semantic.com#StringsDrawn -->

    <owl:Class rdf:about="http://ipro-semantic.com#StringsDrawn">
        <rdfs:subClassOf rdf:resource="http://ipro-semantic.com#Strings"/>
        <rdfs:comment xml:lang="en">Stringed instrument that are played by drawing the strings.</rdfs:comment>
        <rdfs:label xml:lang="en">Strings drawn</rdfs:label>
    </owl:Class>
    


    <!-- http://ipro-semantic.com#StringsPlucked -->

    <owl:Class rdf:about="http://ipro-semantic.com#StringsPlucked">
        <rdfs:subClassOf rdf:resource="http://ipro-semantic.com#Strings"/>
        <rdfs:comment xml:lang="en">Stringed instruments played by plucking the strings.</rdfs:comment>
        <rdfs:label xml:lang="en">Strings plucked</rdfs:label>
    </owl:Class>
    


    <!-- http://ipro-semantic.com#Synthesizer -->

    <owl:Class rdf:about="http://ipro-semantic.com#Synthesizer">
        <rdfs:subClassOf rdf:resource="http://ipro-semantic.com#Keyboard"/>
        <rdfs:comment xml:lang="en">A synthesizer is an electronic musical instruments that plays sound through electric signals. The sound of a synthesizer comes from an oscillator with audible frequency; the sound can be filtered and modulated.</rdfs:comment>
        <rdfs:label xml:lang="en">Synthesizer</rdfs:label>
    </owl:Class>
    


    <!-- http://ipro-semantic.com#Track -->

    <owl:Class rdf:about="http://ipro-semantic.com#Track">
        <rdfs:subClassOf rdf:resource="http://www.ontologydesignpatterns.org/cp/owl/list.owl#ListItem"/>
        <rdfs:comment xml:lang="en">A track (or song) is a piece of music and element of an album. A track have a duration from 2 minutes or less to 30 minutes, or even fill the whole album.</rdfs:comment>
        <rdfs:label xml:lang="en">Track</rdfs:label>
    </owl:Class>
    


    <!-- http://ipro-semantic.com#Vocals -->

    <owl:Class rdf:about="http://ipro-semantic.com#Vocals">
        <rdfs:subClassOf rdf:resource="http://ipro-semantic.com#MusicalInstrument"/>
        <rdfs:comment xml:lang="en">Part of a piece of music that is sung. Vocals are an ubuquitous element of modern music.</rdfs:comment>
        <rdfs:label xml:lang="en">Vocals</rdfs:label>
    </owl:Class>
    


    <!-- http://ipro-semantic.com#WindInstrument -->

    <owl:Class rdf:about="http://ipro-semantic.com#WindInstrument">
        <rdfs:subClassOf rdf:resource="http://ipro-semantic.com#MusicalInstrument"/>
        <rdfs:comment xml:lang="en">A musical instrument in which sound is produced by the vibration of air, typically by the player blowing into the instrument.</rdfs:comment>
        <rdfs:label xml:lang="en">Wind instrument</rdfs:label>
    </owl:Class>
    


    <!-- http://www.w3.org/2006/time#DurationDescription -->

    <owl:Class rdf:about="http://www.w3.org/2006/time#DurationDescription"/>
</rdf:RDF>



<!-- Generated by the OWL API (version 4.5.9.2019-02-01T07:24:44Z) https://github.com/owlcs/owlapi -->

